Coq/intrusive/trees/map.v
@@ -1,0 +1,72 @@
+From Intrusive Require Import Setup Util bst.
+
+Module Map.
+Section Map.
+  Context `{!heapGS Σ}.
+
+(* ------------------ Representation predicate  ------------------- *)
+
+(* Map that assigns a value to every key *)
+Definition pred (l: loc)(m: gmap nat val) : iProp Σ :=
+  ∃ m', Tree.is_Intrusive_Map l m'
+∗ [∗ map] l ; v ∈ m' ; m, (l +ₗ -1) ↦ v.
+
+Notation is_Map := pred.
+
+(* --------------------- Functions on Maps ---------------------- *)
+
+Definition emptymap : val :=
+  λ: "<>",
+    let: "new" := AllocN #1 NONEV in
+    Tree.new "new";; "new".
+
+Definition insert : val :=
+  λ: "map" "k" "v",
+    let: "new_node" := AllocN #4 NONEV in
+    "new_node"      <- "v" ;;
+    "new_node" +ₗ #3 <- "k" ;;
+    let: "ml" := Tree.insert "map" ("new_node" +ₗ #1) in
+    match: "ml" with
+      NONE      => #()
+    | SOME "l'" => array_free "l'" #3 
+    end.
+
+Definition lookup : val :=
+  λ: "map" "k",
+    let: "pos" := Tree.locate "map" "k" in
+    !("pos" +ₗ #-1).
+
+(* -------------- Verification of the Specifications -------------- *)
+
+Lemma emptymap_spec :
+  {{{ emp }}}
+    emptymap #()
+  {{{ l, RET #l; is_Map l ∅ }}}.
+Proof.
+  iSteps as (Φ l) "HΦ Hl"; iModIntro.
+  wp_apply (Tree.new_spec with "[$Hl]"); iSteps.
+  iExists ∅. iSplitL.
+  { now iApply Tree.Intrusive_Map_empty. }
+  now iApply big_sepM2_empty.
+Qed.
+
+Lemma insert_spec (l: loc) m (k: nat) (v: val) :
+  {{{ is_Map l m }}}
+    insert #l #k v
+  {{{ RET #(); is_Map l (<[k := v]> m) }}}.
+Proof.
+  iSteps as (Φ m' p) "Hl Hmap HΦ H0 H12 H3".
+  rewrite unfold_array; simpl.
+  iDestruct "H12" as "[H1 H2]".
+  wp_apply (Tree.insert_spec_Intrusive_Map with "[$Hl H1 H2 H3]"); first iSteps.
+  destruct (m' !! k) as [l'|].
+  - iSteps as (v1 v2) "Hl Hl'"; iModIntro.
+    wp_apply (wp_array_free with "[$Hl'] [-]"); first (simpl; lia); iSteps.
+    iApply (big_sepM2_insert_2 with "[H0] [Hmap]"); iSteps.
+  - iSteps; iModIntro.
+    iApply (big_sepM2_insert_2 with "[H0] [Hmap]"); iSteps.
+Qed.
+
+
+End Map.
+End Map.
